\subsection{}
\begin{math}
    A=\begin{pmatrix}
        1 & -5\\
        4 & 3
    \end{pmatrix}
    \hspace{6px}
    B=\begin{pmatrix}
        2 & -2\\
        4 & 1
    \end{pmatrix}
    \hspace{6px}
    C=\begin{pmatrix}
        1 & 0 & -2\\
        -3 & 4 & 0\\
        7 & 2 & 5
    \end{pmatrix}
    \hspace{6px}
    D=\begin{pmatrix}
        -4 & 5 & 6\\
        -2 & 3 & 1\\
        0 & 9 & 3
    \end{pmatrix}
\end{math}
\begin{enumerate}
    \item[a)]
        \begin{math}
            AB=\begin{pmatrix}
                -18 & -7\\
                20 & -5
            \end{pmatrix}
            \hspace{6px}
            BA=\begin{pmatrix}
                -6 & -16\\
                8 & -17
            \end{pmatrix}
            \hspace{6px}
            A^2=\begin{pmatrix}
                -19 & -20\\
                16 & -11
            \end{pmatrix}
            \hspace{6px}
            \text{BC Ã¤r ej definierad}
            \hspace{6px}
            CD=\begin{pmatrix}
                -4 & -13 & 0\\
                4 & -3 & -14\\
                -32 & 86 & 59
            \end{pmatrix}
            \hspace{6px}
            DC=\begin{pmatrix}
                23 & 32 & 38\\
                -4 & 14 & 9\\
                -6 & 42 & 15
            \end{pmatrix}
        \end{math}
    \item[b)]
        \begin{math}
            A(A+B)=A^2+AB=\begin{pmatrix}
                -37 & -27\\
                36 & -16
            \end{pmatrix}
        \end{math}
    \item[c)]
        \begin{math}
            A(BA)=(AB)A=\begin{pmatrix}
                -46 & 69\\
                0 & -115
            \end{pmatrix}
        \end{math}
\end{enumerate}