\subsection{}
\begin{math}
    A=\begin{pmatrix}
        1 & -5\\
        4 & 3
    \end{pmatrix}
    \hspace{6px}
    B=\begin{pmatrix}
        2 & -2\\
        4 & 1
    \end{pmatrix}
    \hspace{6px}
    C=\begin{pmatrix}
        1 & 0 & -2\\
        -3 & 4 & 0\\
        7 & 2 & 5
    \end{pmatrix}
    \hspace{6px}
    D=\begin{pmatrix}
        -4 & 5 & 6\\
        -2 & 3 & 1\\
        0 & 9 & 3
    \end{pmatrix}
\end{math}
\begin{enumerate}
    \item[a)]
        \begin{math}
            A^T=\begin{pmatrix}
                1 & 4\\
                -5 & 3
            \end{pmatrix}
            \hspace{6px}
            B^T=\begin{pmatrix}
                2 & 4\\
                -2 & 1
            \end{pmatrix}
            \hspace{6px}
            C^T=\begin{pmatrix}
                1 & -3 & 7\\
                0 & 4 & 2\\
                -2 & 0 & 5
            \end{pmatrix}
            \hspace{6px}
            D^T=\begin{pmatrix}
                -4 & -2 & 0\\
                5 & 3 & 9\\
                6 & 1 & 3
            \end{pmatrix}
        \end{math}
    \item[b)]
        Ingen
    \item[c)]
        \begin{math}
            (AB)^T=\begin{pmatrix}
                -18 & 20\\
                -7 & -5
            \end{pmatrix}
            \hspace{6px}
            A^TB^T=\begin{pmatrix}
                -6 & 8\\
                -16 & -17
            \end{pmatrix}
            =(BA)^T
            \hspace{6px}
            B^TA^T=(AB)^T=\begin{pmatrix}
                -18 & 20\\
                -7 & -5
            \end{pmatrix}
        \end{math}
\end{enumerate}