\subsection{}
\begin{math}
    A=\begin{pmatrix}
        1 & -5\\
        4 & 3
    \end{pmatrix}
    \hspace{6px}
    B=\begin{pmatrix}
        2 & -2\\
        4 & 1
    \end{pmatrix}
    \hspace{6px}
    C=\begin{pmatrix}
        1 & 0 & -2\\
        -3 & 4 & 0\\
        7 & 2 & 5
    \end{pmatrix}
    \hspace{6px}
    D=\begin{pmatrix}
        -4 & 5 & 6\\
        -2 & 3 & 1\\
        0 & 9 & 3
    \end{pmatrix}
\end{math}
\begin{enumerate}
    \item[a)]
        \begin{math}
            A+B
            =\begin{pmatrix}
                3 & -7\\
                8 & 3
            \end{pmatrix}
            \\
            \text{B+C Ã¤r ej definierad}
            \\
            C+D
            =\begin{pmatrix}
                -3 & 5 & 4\\
                -5 & 7 & 1\\
                7 & 11 & 8
            \end{pmatrix}
            \\
            -3C
            =\begin{pmatrix}
                -3 & 0 & 6\\
                9 & -12 & 0\\
                -21 & -6 & -15
            \end{pmatrix}
            \\
            2A+B
            =\begin{pmatrix}
                4 & -12\\
                12 & 7
            \end{pmatrix}
        \end{math}
    \item[b)]
        \begin{math}
            X
            =\frac{1}{2}(5B-3A)
            =\frac{1}{2}\begin{pmatrix}
                7 & 5\\
                8 & -4
            \end{pmatrix}
        \end{math}
\end{enumerate}