\subsection{}
\begin{math}
    C=\begin{pmatrix}
        1 & 0 & -2\\
        -3 & 4 & 0\\
        7 & 2 & 5
    \end{pmatrix}
    \hspace{6px}
    D=\begin{pmatrix}
        -4 & 5 & 6\\
        -2 & 3 & 1\\
        0 & 9 & 3
    \end{pmatrix}
    \hspace{6px}
    u=\begin{pmatrix}
        2\\
        4\\
        1
    \end{pmatrix}
    \hspace{6px}
    v=\begin{pmatrix}
        -2\\
        3\\
        1
    \end{pmatrix}
\end{math}
\begin{enumerate}
    \item[a)]
        \begin{math}
            Cu
            =\begin{pmatrix}
                0\\
                10\\
                27
            \end{pmatrix}
            \hspace{6px}
            C(2u)
            =\begin{pmatrix}
                0\\
                20\\
                54
            \end{pmatrix}
        \end{math}
    \item[b)]
        \begin{math}
            D(u+v)
            =Du+Dv
            =\begin{pmatrix}
                47\\
                23\\
				69
            \end{pmatrix}
        \end{math}
    \item[c)]
        \begin{math}
			(C+D)v
			=Cv+Dv
			=\begin{pmatrix}
				25\\
				32\\
				27
			\end{pmatrix}
        \end{math}
\end{enumerate}