\subsection{}
\begin{math}
    v
    =\begin{pmatrix}
        1\\
        4\\
        -3
    \end{pmatrix},
    \hspace{6px}
    w
    =\begin{pmatrix}
        2\\
        -1\\
        0
    \end{pmatrix}
\end{math}
\begin{enumerate}
    \item[a)]
        \begin{math}
            v\cdot w
            =1*2+4*(-1)+(-3)*0
            =2-4+0
            =-2
        \end{math}
    \item[b)]
        \begin{math}
            v_{L}
            =\frac{w\cdot v}{w\cdot w}w
            =\frac{-2}{5}w
            =\frac{-2}{5}\begin{pmatrix}
                2\\
                -1\\
                0
            \end{pmatrix}
        \end{math}
    \item[c)]
        \begin{math}
            v_{S}
            =2v_{L}-v
            =2\frac{w\cdot v}{w\cdot w}w-v
            =\frac{-4}{5}w-v
            =\frac{-4}{5}\begin{pmatrix}
                2\\
                -1\\
                0
            \end{pmatrix}-\begin{pmatrix}
                1\\
                4\\
                -3
            \end{pmatrix}
            =\begin{pmatrix}
                \frac{-8}{5}\\
                \frac{4}{5}\\
                0
            \end{pmatrix}-\begin{pmatrix}
                1\\
                4\\
                -3
            \end{pmatrix}
            =\begin{pmatrix}
                \frac{-8}{5}-1\\
                \frac{4}{5}-4\\
                0+3
            \end{pmatrix}
            =\begin{pmatrix}
                \frac{-13}{5}\\
                \frac{-16}{5}\\
                3
            \end{pmatrix}
            =\begin{pmatrix}
                \frac{-13}{5}\\
                \frac{-16}{5}\\
                \frac{15}{5}
            \end{pmatrix}
            =\frac{1}{5}\begin{pmatrix}
                -13\\
                -16\\
                15
            \end{pmatrix}
        \end{math}
\end{enumerate}