\subsection{}
\begin{math}
	P=(1, -4, -3),
	\hspace{6px}
	Q=(-2 -6, 1),
	\hspace{6px}
	R=(5, 1, -1),
	\hspace{6px}
	S=(2, -1, 3)
\end{math}
\begin{enumerate}
	\item[a)]
		\begin{math}
			\vec{PQ}
			=\begin{pmatrix}
				(-2)-1\\
				(-6)-(-4)\\
				1-(-3)
			\end{pmatrix}
			=\begin{pmatrix}
				-3\\
				-2\\
				4
			\end{pmatrix}
			\\
			\vec{SR}
			=\begin{pmatrix}
				5-2\\
				1-(-1)\\
				(-1)-3
			\end{pmatrix}
			=\begin{pmatrix}
				3\\
				2\\
				-4
			\end{pmatrix}
			\\
			\vec{QS}
			=\begin{pmatrix}
				2-(-2)\\
				(-1)-(-6)\\
				3-1
			\end{pmatrix}
			=\begin{pmatrix}
				4\\
				5\\
				2
			\end{pmatrix}
		\end{math}
	\item[b)]
		\begin{math}
			2\vec{PQ}+3\vec{SR}
			=2\begin{pmatrix}
				-3\\
				-2\\
				4
			\end{pmatrix}
			+3\begin{pmatrix}
				3\\
				2\\
				-4
			\end{pmatrix}
			=\begin{pmatrix}
				-6\\
				-4\\
				8
			\end{pmatrix}
			+\begin{pmatrix}
				9\\
				6\\
				-12
			\end{pmatrix}
			=\begin{pmatrix}
				(-6)+9\\
				(-4)+6\\
				8-12
			\end{pmatrix}
			=\begin{pmatrix}
				3\\
				2\\
				-4
			\end{pmatrix}
			=\vec{SR}
			\\
			3\vec{RS}-\vec{QS}
			=3\begin{pmatrix}
				-3\\
				-2\\
				4
			\end{pmatrix}
			-\begin{pmatrix}
				4\\
				5\\
				2
			\end{pmatrix}
			=\begin{pmatrix}
				-9\\
				-6\\
				12
			\end{pmatrix}
			-\begin{pmatrix}
				4\\
				5\\
				2
			\end{pmatrix}
			=\begin{pmatrix}
				(-9)-4\\
				(-6)-5\\
				12-2
			\end{pmatrix}
			=\begin{pmatrix}
				-13\\
				-11\\
				10
			\end{pmatrix}
		\end{math}
	\item[c)]
		\begin{math}
			\vec{PQ}=\vec{RS}
			\\
			\vec{QS}=\vec{PR}
		\end{math}
\end{enumerate}