\subsection{}
\begin{math}
    \begin{cases}
        x=2+t\\
        y=2+2t\\
        z=3+3t
    \end{cases}
    \hspace{6px}
    v=\begin{pmatrix}
        1\\
        2\\
        3
    \end{pmatrix}
    \hspace{6px}
    P_0=(2,2,3)
    \\
    s=\vec{P_0O}=\begin{pmatrix}
        -2\\
        -2\\
        -3
    \end{pmatrix}
    \\
    n
    =v\times s
    =\begin{pmatrix}
        0\\
        -3\\
        2
    \end{pmatrix}
    \\
    n\cdot v
    =0*1+(-3)*2+2*3
    =0-6+6
    =0
    \\
    n\cdot s
    =0*(-2)+(-3)*(-2)+2*(-3)
    =0+6-6
    =0
    \\
    -3y+2z=0
\end{math}