\subsection{}
\begin{math}
    v=
    \begin{pmatrix}
        1\\
        4\\
        -3
    \end{pmatrix}
\end{math}
\begin{enumerate}
    \item[a)]
        \begin{math}
            ||v||
            =\sqrt{v\cdot v}
            =\sqrt{1^2+4^2+(-3)^2}
            =\sqrt{1+16+9}
            =\sqrt{26}
            \\
            v_{e1}
            =\frac{1}{\sqrt{26}}\begin{pmatrix}
                1\\
                4\\
                -3
            \end{pmatrix},
            \hspace{6px}
            v_{e2}
            =\frac{1}{\sqrt{26}}\begin{pmatrix}
                -1\\
                -4\\
                3
            \end{pmatrix},
        \end{math}
        \hspace{6px}
		Nej!
    \item[b)]
    \begin{math}
        w
        =v\times \begin{pmatrix}
            0\\
            0\\
            1
        \end{pmatrix}
        =\begin{pmatrix}
            4*1-(-3)*0\\
            (-3)*0-1*1\\
            1*0-4*0
        \end{pmatrix}
        =\begin{pmatrix}
            4-0\\
            0-1\\
            0-0
        \end{pmatrix}
        =\begin{pmatrix}
            4\\
            -1\\
            0
        \end{pmatrix}
        \\
        ||w||
        =\sqrt{4^2+(-1)^2}
        =\sqrt{16+1}
        =\sqrt{17}
        \\
        w_{e1}
        =\frac{1}{\sqrt{17}}\begin{pmatrix}
            4\\
            -1\\
            0
        \end{pmatrix}
        \\
        w_{e2}
        =\frac{1}{\sqrt{17}}\begin{pmatrix}
            -4\\
            1\\
            0
        \end{pmatrix}
    \end{math}
    \hspace{6px}
    Ja!
    \item[c)]
        \begin{math}
            ||v||
            =\sqrt{v\cdot v}
            =\sqrt{1^2+4^2+(-3)^2}
            =\sqrt{1+16+9}
            =\sqrt{26}
            \\
            w
            =\frac{7}{\sqrt{26}}\begin{pmatrix}
                1\\
                4\\
                -3
            \end{pmatrix},
        \end{math}
\end{enumerate}