\subsection{}
\begin{math}
    ||u||=1, 
	\hspace{6px}
    ||v||=1,
	\hspace{6px}
    \theta=\pi/3
\end{math}
\begin{enumerate}
    \item[a)]
        \begin{math}
            u\cdot v
            =||u||*||v||*\cos(\theta)
            =1*1*\cos(\pi/3)
            =\cos(\pi/3)
            =\frac{1}{2}
        \end{math}
    \item[b)]
        \begin{math}
            (3u-4v)\cdot (u+5v)
            =3u\cdot u+3u\cdot 5v+(-4)v\cdot u+(-4)v\cdot 5v
            =3(u\cdot u)+15(u\cdot v)-4(v\cdot u)-20(v\cdot v)
            =3*1+15*0.5-4*0.5-20*1
            =3+7.5-2-20
            =\frac{6}{2}+\frac{15}{2}-\frac{4}{2}-\frac{40}{2}
            =\frac{-23}{2}
        \end{math}
    \item[c)]
        \begin{math}
            ||3u+4v||
			=\sqrt{(3u+4v)\cdot (3u+4v)}
			=\sqrt{3u\cdot 3u+3u\cdot 4v + 4v\cdot 3u + 4v\cdot 4v}
			=\sqrt{9(u\cdot u)+12(u\cdot v)+12(v\cdot u) + 16(v\cdot v)}
			=\sqrt{9*1+12\frac{1}{2}+12\frac{1}{2}+16*1}
			=\sqrt{9+6+6+16}
			=\sqrt{37}
        \end{math}
    \item[d)]
        \begin{math}
			(u\cdot v)v
			=\frac{1}{2}v
        \end{math}
\end{enumerate}