\subsection{}
\begin{math}
	v
	=\begin{pmatrix}
		5\\
		-7
	\end{pmatrix}
\end{math}
\begin{enumerate}
	\item[a)]
		\begin{math}
			||v||
			=\sqrt{v\cdot v}
			=\sqrt{5^2+(-7)^2}
			=\sqrt{25+49}
			=\sqrt{74}
			\\
			v_{e1}
			=\frac{1}{\sqrt{74}}\begin{pmatrix}
				5\\
				-7
			\end{pmatrix},
            \hspace{6px}
			v_{e2}
			=\frac{1}{\sqrt{74}}\begin{pmatrix}
				-5\\
				7
			\end{pmatrix},
		\end{math}
		\hspace{6px}
		Nej!
	\item[b)]
		\begin{math}
            ||v||
			=\sqrt{v\cdot v}
			=\sqrt{5^2+(-7)^2}
			=\sqrt{25+49}
			=\sqrt{74}
			\\
			v_{e1}
			=\frac{1}{\sqrt{74}}\begin{pmatrix}
				7\\
				5
			\end{pmatrix},
            \hspace{6px}
			v_{e2}
			=\frac{1}{\sqrt{74}}\begin{pmatrix}
				-7\\
				-5
			\end{pmatrix},
		\end{math}
		\hspace{6px}
		Nej!
	\item[c)]
		\begin{math}
            ||w||=2,
            \hspace{6px}
            ||v||
			=\sqrt{v\cdot v}
			=\sqrt{5^2+(-7)^2}
			=\sqrt{25+49}
			=\sqrt{74}
			\\
			w
			=\frac{2}{\sqrt{74}}\begin{pmatrix}
				5\\
				-7
			\end{pmatrix}
		\end{math}
\end{enumerate}